\section{Differential Geometry}

\subsection{Conventions}
We adopt the following conventions and normalizations for form fields

\begin{align}
F &\equiv \frac{1}{p!}F_{\mu_1...\mu_p} dx^{\mu_1}...dx^{\mu_p}\\
F_{\mu_1...\mu_p} &\equiv F_{[\mu_1...\mu_p]}\\
|F|^2 &\equiv \frac{1}{p!}F_{\mu_1...\mu_p} F^{\mu_1...\mu_p}=\frac{1}{p!}F^2\\
(d F)_{\mu_1...\mu_{p+1}} &= (p+1)\partial_{[\mu_1} F_{\mu_2...\mu_{p+1}]}\\
(F^{(p)} \wedge G^{(q)})_{\mu_1...\mu_p \nu_1 ... \nu_q}
&=\frac{(p+q)!}{p!q!}F^{(p)}_{[\mu_1...\mu_p}  G^{(q)}_{\nu_1 ... \nu_q]}
\end{align}
We will use $\epsilon_{\mu_1 ... \mu_p}$ to denote the Levi-Civita tensor and $\varepsilon_{\mu_1 ... \mu_p}$ to denote the flat-space fully antisymmetrized symbol.


\begin{equation}
\epsilon_{\mu_1...\mu_D} = \sqrt{|g|}\varepsilon_{\mu_1...\mu_D},\quad
\varepsilon_{0,1,...,(D-2),(D-1)} = 1,
\end{equation}


\begin{equation}
\epsilon_{\mu_1...\mu_p \lambda_1 ...\lambda_{D-p}}
\epsilon^{\nu_1...\nu_p \lambda_1 ...\lambda_{D-p}}
=(-1)^{[t]} p!(D-p)!\delta^{\nu_1...\nu_p}_{\mu_1...\mu_p}
\end{equation}


\begin{equation}
(*A)_{\mu_1...\mu_{D-p}} = \frac{1}{p!}
\epsilon_{\mu_1...\mu_{D-p}}{}^{\nu_1...\nu_p} A_{\nu_1...\nu_p},
\end{equation}

\subsection{Useful forms identities}

One can then show that
\begin{equation}
*(*A) = (-1)^{[t]}(-1)^{p(D-p)}A,
\end{equation}
\begin{equation}
(*F)\wedge *(*F)=(-1)^{[t]}F\wedge *F,\quad
|*F|^2 = (-1)^{[t]}|F|^2
\end{equation}
as well as
\begin{equation}
\frac{1}{(D-p-1)!}(*F)_{\mu ...}(*F)_\nu{}^{...}
=(-1)^{[t]}\left[
    \frac{1}{p!}F^2 g_{\mu\nu} - \frac{1}{(p-1)!}F_{\mu...}F_\nu{}^{...}
\right]
\end{equation}
\begin{proof}
\begin{equation}
\begin{aligned}
\frac{1}{(D-p-1)!}(*F)_{\mu ...}(*F)_\nu{}^{...}
&=\frac{1}{(D-p-1)!}\frac{1}{p!p!}
\epsilon_{\mu \mu_1...\mu_p \lambda_1...\lambda_{D-p-1}}
\epsilon_{\nu} {}^{\nu_1...\nu_p} {}^{\lambda_1...\lambda_{D-p-1}}
F^{\mu_1...\mu_p}F_{\nu_1...\nu_p}\\
&=\frac{p+1}{p!}(-1)^{[t]} g_{\nu\rho} \delta^{[\rho \nu_1...\nu_p]}_{[\mu \mu_1...\mu_p]}F^{\mu_1...\mu_p}F_{\nu_1...\nu_p}
\end{aligned}
\end{equation}
The term $\delta^{[\rho \nu_1...\nu_p]}_{[\mu \mu_1...\mu_p]}$
has in total $(p+1)!(p+1)!$ terms and is thus normalized by such number. Within those terms, $(p+1)p!p!$ of which give 
$\delta^{\rho}_{\mu} \delta^{\nu_1...\nu_p}_{\mu_1...\mu_p}$
equivalent and $(p+1)(p)p!p!$ give $
-\delta^{\rho}_{\mu_1}\delta^{\nu_1...\nu_p}_{ \mu ...\mu_p}$
equivalent, hence the relation provided.
\end{proof}
As a corollary, one can show suppose $S_{MN}$ is defined by
\begin{equation}
S_{MN}\big|_{F}\equiv
\frac{1}{2}\left[
    \frac{1}{(n-1)!}F_{M...}F_N^{...}
    -\frac{n-1}{D-2}\left(\frac{1}{n!}F^2\right)g_{MN}
\right],
\end{equation}
then
\begin{equation}
S_{MN}|_{*F} = -(-1)^{[t]}S_{MN}|_{F}.
\end{equation}


\subsection{Useful gravity identities}

Under dilatation, the Ricci tensor transforms as
\begin{equation}
R(\Lambda^2 g_{mn})
=\Lambda^{-2}[R-2(d-1)\nabla^2\ln\Lambda - (d-2)(d-1)(\nabla \ln \Lambda)^2].
\end{equation}
For a brane-like metric
\begin{equation}
ds_D^2 = H^{a}ds_{d}^2 + H^bds_{D-2}^2,
\end{equation}
and $H\equiv H(r)$ with $r\equiv \sqrt{y^my^m}$ is a harmonic function in $(D-d)$-dimensions, usually taken to be
\begin{equation}
H = 1 + \frac{Q}{r^{\tilde{d}}},\quad \tilde{d} = D-d-2,
\end{equation}
The Ricci tensor is found to be
\begin{equation}
\begin{aligned}
R_{\mu\nu}
&=-\eta_{\mu\nu}(H')^2H^{a-b-2}\left[\frac{a(ad+b\tilde d-2)}{4}\right]\\
R_{mn} 
&= \frac{(H')^2}{4H^2}\left[-b(ad+b\tilde{d}-2)\delta_{mn}-\frac{y^m y^n}{r^2}\left[ad(a-b)-(ad+b\tilde{d})(b+2)\right]\right]\\
&+\frac{H'}{rH}\frac{(ad+b\tilde{d})}{2}\left[-\delta_{mn} + \frac{y^m y^n}{r^2}(2+\tilde{d})\right].
\end{aligned}
\end{equation}
Usually one adopts the ansatz that $A_{n-1} \propto H$, hence $F_n \propto H'$.
Then the energy-momentum tensor will be exactly quadratic in $H'$ up to some powers of $H$.
This demands
\begin{equation}
b=-ad/\tilde{d},
\end{equation}
and we can write down a simplified Ricci tensor
\begin{equation}
\begin{aligned}
R_{\mu\nu} 
&= \frac{a}{2}(H')^2H^{a-b-2} \eta_{\mu\nu}
=\frac{a}{2}(H')^2H^{\frac{ad+(a-2)(D-d-2)}{(D-d-2)}} \eta_{\mu\nu},\\
R_{mn}
&=\frac{(H')^2}{4H^2}\left[2b\delta_{mn}-ad(a-b)\frac{y^my^n}{r^2}\right]
=-\frac{ad}{2(D-d-2)}\frac{(H')^2}{H^2}\left[
\delta_{mn}+\frac{a(D-2)}{2}\frac{y^m y^n}{r^2}
\right].
\end{aligned}
\end{equation}
